CollapsingTowers/TwoLevelFinal/Defs.lean
@@ -4,3 +4,4 @@ import CollapsingTowers.TwoLevelFinal.OperationalSemantics.Defs
 import CollapsingTowers.TwoLevelFinal.SyntacticTyping.Defs
 import CollapsingTowers.TwoLevelFinal.SyntacticSoundness.Defs
 import CollapsingTowers.TwoLevelFinal.CtxEquiv.Defs
+import CollapsingTowers.TwoLevelFinal.LogicalEquiv.Defs
