CollapsingTowers/TwoLevelFinal/LogicalEquiv/Defs.lean
@@ -1,0 +1,2 @@
+import CollapsingTowers.TwoLevelFinal.LogicalEquiv.World
+import CollapsingTowers.TwoLevelFinal.LogicalEquiv.LogicalRelation
