CollapsingTowers/TwoLevelFinal/LogicalEquiv/LogicalRelation.lean
@@ -1,0 +1,21 @@
+import CollapsingTowers.TwoLevelFinal.SyntacticSoundness.Defs
+import CollapsingTowers.TwoLevelFinal.LogicalEquiv.World
+
+-- (σ₀, σ₁) : 𝓦 ≜ ∀ 𝓦(l₀, l₁). σ₀(l₁) = σ₀(l₁)
+@[simp]
+def log_well_store (𝓦 : World) (σ₀ σ₁ : Store) : Prop :=
+  PartialBijection 𝓦 ∧ (
+  ∀ l₀ l₁,
+    𝓦 l₀ l₁ →
+    ∃ n,
+      binds l₀ (.lit n) σ₀ ∧
+      binds l₁ (.lit n) σ₁
+  )
+
+abbrev KripkeWorld := Nat × World
+
+@[simp]
+def KripkeWorld.future : KripkeWorld → KripkeWorld → Prop :=
+  fun (k, 𝓦₀) (j, 𝓦₁) => j ≤ k ∧ 𝓦₁ ⊒ 𝓦₀
+
+notation:max 𝓦₁ " ⊇ " 𝓦₀  => KripkeWorld.future 𝓦₀ 𝓦₁
